perfecting new poly and its operations, update project to fit new poly

code/PolyAB.v
@@ -7,21 +7,22 @@ Open Scope Z.
 Module Polynomial.
 Import Assertion_D.
 
-Definition poly := list Z. (* The power decreases as the index goes up *)
+(** Definitions of poly *)
+Definition poly := list Z. (* The power increases as the index goes up *)
+
+Definition ZERO : poly := nil.
+Definition CONSTANT : poly := 1::nil.
+Definition LINEAR : poly := 0::1::nil.
+Definition QUADRATIC : poly := 0::0::1::nil.
+Definition CUBIC : poly := 0::0::0::1::nil.
+(** [] *)
 
 (** Evaluations of polynomial *)
-Fixpoint poly_eval (p : poly) : Z -> Z :=
-  fun z =>
+Fixpoint poly_eval (p : poly) : Z -> Z := 
+  fun z => 
     match p with
     | nil => 0
-    | h :: t => h * (Z.pow z (Z.of_nat (length t))) + (poly_eval t z)
-    end.
-    
-Fixpoint poly_eval' (p' : poly) : Z -> Z := 
-  fun z => 
-    match p' with
-    | nil => 0
-    | h :: t' => h + z * (poly_eval' t' z)
+    | h :: t => h + z * (poly_eval t z)
     end.
 
 Open Scope term_scope.
@@ -37,395 +38,277 @@ Fixpoint poly_eval_lv (p : poly) : logical_var -> term :=
   fun v =>
     match p with
     | nil => 0
-    | h :: t => h * (TPower v (length t)) + (poly_eval_lv t v)
+    | h :: t => h + v * (poly_eval_lv t v)
     end.
 
 Close Scope term_scope.
 (** [] *)
 
 (** Operations of polynomial *)
-Fixpoint poly_add_body (l1 l2 : list Z) : list Z :=
-  match l1, l2 with
-  | nil, nil => l2
+Fixpoint poly_add (p1 p2 : poly) : poly :=
+  match p1, p2 with
+  | nil, nil => nil
   | h::t, nil => h::t
   | nil, h::t => h::t
-  | h::t, h'::t' => (h+h')::(poly_add_body t t')
+  | h::t, h'::t' => (h+h')::(poly_add t t')
   end.
 
-Definition poly_add (p1 p2 : poly) : poly := rev (poly_add_body (rev p1) (rev p2)).
-
-Fixpoint poly_mult (p1 p2 : poly) : poly :=
-  match p1 with
-  | nil => nil
-  | h :: t => poly_add (app p2 (repeat 0 (length t))) (poly_mult t p2)
-  end.
-
-Fixpoint trim_0_l (p : poly) : poly :=
+Fixpoint trim_0 (p : poly) : poly :=
   match p with
   | nil => nil
-  | h :: t => if Z.eq_dec h 0 then trim_0_l t else h :: t
+  | h :: t => match trim_0 t with
+              | nil => if Z.eq_dec h 0 then nil else h :: nil
+              | _ => h :: trim_0 t
+              end
   end.
 
-Theorem trim_invar:
-  forall p n,
-  poly_eval (trim_0_l p) n = poly_eval p n.
+Fixpoint poly_scalar_mult (k : Z) (p : poly) : poly :=
+  match p with
+  | nil => nil
+  | h :: t => k * h :: poly_scalar_mult k t
+  end.
+
+Fixpoint poly_mult (p1 p2 : poly) : poly := 
+  match p1, p2 with
+  | nil, _ => nil
+  | _, nil => nil
+  | h :: t, _ => poly_add (poly_scalar_mult h p2) (0 :: (poly_mult t p2))
+  end.
+
+Notation "p '+++' q" := (poly_add p q) (at level 60).
+Notation "k ** p" := (poly_scalar_mult k p) (at level 60).
+Notation "p '***' q" := (poly_mult p q) (at level 60).
+
+Section Examples.
+
+Example poly_add_eg : poly_eval ((CONSTANT +++ LINEAR) +++ (CONSTANT +++ QUADRATIC)) 2 = 8.
 Proof.
-  intros p.
-  induction p.
-  - intros. simpl. reflexivity.
-  - intros.
-    simpl. destruct (Z.eq_dec a 0) eqn:eq.
-    + pose proof IHp n.
-      rewrite H. rewrite e.
-      simpl. reflexivity.
-    + simpl. reflexivity.
+  simpl. reflexivity.
 Qed.
 
-Definition highest_nonneg (p : poly) : Prop :=
-  match trim_0_l p with
-  | nil => True
-  | h :: t => h >= 0
-  end.
+Example poly_mult_eg : poly_eval ((CONSTANT +++ LINEAR) *** (CONSTANT +++ QUADRATIC)) 2 = 15.
+Proof.
+  simpl. reflexivity.
+Qed.
+
+End Examples.
 (** [] *)
 
-Example poly_add_eg : poly_eval (poly_add (1::1::nil) (1::0::1::nil)) 2 = 8.
+(** Properties of Shorthand Notations *)
+Fact CONSTANT_spec : forall z, poly_eval CONSTANT z = 1.
 Proof.
-  simpl. reflexivity.
+  intros.
+  simpl.
+  rewrite Z.mul_0_r.
+  reflexivity.
 Qed.
 
-Example poly_mult_eg : poly_eval (poly_mult (1::1::nil) (1::0::1::nil)) 2 = 15.
+Fact LINEAR_spec : forall z, poly_eval LINEAR z = z.
 Proof.
-  simpl. reflexivity.
+  intros.
+  simpl.
+  rewrite Z.mul_0_r.
+  omega.
 Qed.
+
+Fact QUADRATIC_spec : forall z, poly_eval QUADRATIC z = z*z.
+Proof.
+  intros.
+  simpl.
+  rewrite Z.mul_0_r.
+  ring.
+Qed.
+
+Fact CUBIC_spec : forall z, poly_eval CUBIC z = z*z*z.
+Proof.
+  intros.
+  simpl.
+  rewrite Z.mul_0_r.
+  ring.
+Qed.
+(** [] *)
 
 (** Properties of Polynomial Operations *)
-Lemma poly_add_body_empty_r : forall l, poly_add_body l nil = l.
-Proof.
-  intros.
-  destruct l.
-  - auto.
-  - simpl. reflexivity.
-Qed.
-
-Lemma poly_add_empty_r : forall p, poly_add p nil = p.
+Lemma poly_add_nil_l : forall p, poly_add nil p = p.
 Proof.
   intros.
   destruct p.
   - auto.
-  - unfold poly_add.
-    rewrite poly_add_body_empty_r.
-    apply rev_involutive.
-Qed.
-
-Lemma poly_add_body_empty_l : forall l, poly_add_body nil l = l.
-Proof.
-  intros.
-  destruct l.
-  - auto.
   - simpl. reflexivity.
 Qed.
 
-Lemma poly_add_empty_l : forall p, poly_add nil p = p.
+Lemma poly_add_nil_r : forall p, poly_add p nil = p.
 Proof.
   intros.
   destruct p.
   - auto.
-  - unfold poly_add.
-    rewrite poly_add_body_empty_l.
-    apply rev_involutive.
-Qed.
-
-Lemma poly_eval_0s: forall times n,
-  poly_eval (repeat 0 times) n = 0.
-Proof.
-  intros.
-  induction times.
   - simpl. reflexivity.
-  - simpl. omega.
 Qed.
 
-Lemma poly_cons_eval_comm : forall p z n,
-  poly_eval (cons z p) n = poly_eval (cons z (repeat 0 (length p))) n + poly_eval p n.
-Proof.
-  intros.
-  simpl.
-  assert (Datatypes.length (repeat 0 (Datatypes.length p)) = Datatypes.length p).
-  { induction p.
-    - simpl. reflexivity.
-    - simpl. rewrite IHp. reflexivity.
-  }
-  rewrite H.
-  pose proof poly_eval_0s (Datatypes.length p) n.
-  rewrite H0.
-  omega.
-Qed.
-
-Lemma poly_app_eval_comm: forall p1 p2 n,
-  poly_eval (p1 ++ p2) n = poly_eval (p1 ++ (repeat 0 (length p2))) n + poly_eval p2 n.
-Proof.
-  intros.
-  induction p1.
-  - simpl. Search (nil ++ _).
-    pose proof app_nil_l p2.
-    rewrite <- H. simpl.
-    pose proof poly_eval_0s (Datatypes.length p2) n.
-    rewrite H0.
-    omega.
-  - pose proof poly_cons_eval_comm.
-    simpl.
-    assert (Datatypes.length (p1 ++ repeat 0 (Datatypes.length p2)) = Datatypes.length (p1 ++ p2)).
-    { clear IHp1 H.
-      Search (length (_ ++ _)).
-      assert (Datatypes.length (repeat 0%Z (Datatypes.length p2)) = Datatypes.length p2).
-      { induction p2.
-        - simpl. reflexivity.
-        - simpl. rewrite IHp2. reflexivity.
-      }
-      pose proof app_length p1 p2.
-      rewrite H0. 
-      pose proof app_length p1 (repeat 0 (Datatypes.length p2)).
-      rewrite H1.
-      rewrite H.
-      omega.
-    }
-    rewrite H0.
-    rewrite IHp1.
-    omega.
-Qed.
-
-Lemma poly_eval_repeat_length_p: forall a (p : poly) z,
-  poly_eval (a :: repeat 0 (length p)) z = a * z ^ (Z.of_nat (length p)).
-Proof.
-  intros.
-  simpl.
-  pose proof poly_eval_0s (length p) z.
-  rewrite H.
-  pose proof repeat_length 0 (length p).
-  rewrite H0.
-  omega.
-Qed.
-
-Theorem poly_eval'_add_body_iso : forall (p1 p2 : poly) (z : Z),
-  poly_eval' (poly_add_body p1 p2) z = poly_eval' p1 z + poly_eval' p2 z.
-Proof.
-  intros.
-  revert p2.
-  induction p1; intros.
-  - rewrite poly_add_body_empty_l. simpl. reflexivity.
-  - induction p2.
-    + simpl. omega.
-    + simpl. specialize (IHp1 p2). rewrite IHp1. 
-      rewrite Z.mul_add_distr_l. omega.
-Qed.
-
-Lemma poly_eval'_cons : forall (p: poly) (a z : Z),
-  poly_eval' (a :: p) z = a + z * (poly_eval' p z).
-Proof.
-  simpl.
-   reflexivity.
-Qed.
-
-Lemma poly_eval'_nil : forall (z : Z),
-  poly_eval' nil z = 0.
+Lemma poly_mult_nil_l : forall p, poly_mult nil p = nil.
 Proof.
   intros.
   simpl.
   reflexivity.
 Qed.
 
-Lemma poly_eval'_app : forall (p1 p2 : poly) (z : Z),
-  poly_eval' (p1 ++ p2) z = poly_eval' p1 z + (z^(Z.of_nat (length p1))) * (poly_eval' p2 z).
+Lemma poly_mult_nil_r : forall p, poly_mult p nil = nil.
+Proof.
+  intros.
+  destruct p; auto.
+Qed.
+
+Lemma poly_eval_zero: forall n z,
+  poly_eval (repeat 0 n) z = 0.
+Proof.
+  intros.
+  induction n.
+  - simpl. reflexivity.
+  - simpl. rewrite IHn. omega.
+Qed.
+
+Theorem poly_add_spec : forall (p1 p2 : poly) (z : Z),
+  poly_eval (poly_add p1 p2) z = poly_eval p1 z + poly_eval p2 z.
+Proof.
+  intro.
+  induction p1; intros.
+  - rewrite poly_add_nil_l. simpl. reflexivity.
+  - destruct p2.
+    + simpl. omega.
+    + simpl. rewrite IHp1.
+      rewrite Z.mul_add_distr_l. omega.
+Qed.
+
+Theorem poly_scalar_mult_spec : forall (k : Z) (p : poly) (z : Z),
+  poly_eval (poly_scalar_mult k p) z = k * poly_eval p z.
+Proof.
+  intros.
+  induction p.
+  - simpl. rewrite Z.mul_0_r. reflexivity.
+  - simpl. rewrite IHp. ring.
+Qed.
+
+Theorem poly_mult_spec : forall (p1 p2 : poly) (z : Z),
+  poly_eval (poly_mult p1 p2) z = poly_eval p1 z * poly_eval p2 z.
+Proof.
+  intro.
+  induction p1; intros.
+  - auto.
+  - destruct p2.
+    + simpl. rewrite Z.mul_0_r. reflexivity.
+    + simpl.
+      rewrite poly_add_spec. rewrite IHp1.
+      rewrite poly_scalar_mult_spec. simpl.
+      ring.
+Qed.
+
+Theorem trim_invar:
+  forall p z,
+  poly_eval (trim_0 p) z = poly_eval p z.
+Proof.
+  intro.
+  induction p; intros.
+  - auto.
+  - simpl.
+    destruct (trim_0 p) eqn:eqp.
+    + destruct (Z.eq_dec a 0) eqn:eqa; rewrite <- IHp; simpl; omega.
+    + rewrite <- eqp in *.
+      simpl. rewrite IHp. reflexivity.
+Qed.
+
+Lemma poly_eval_cons : forall (p: poly) (a z : Z),
+  poly_eval (a :: p) z = a + z * (poly_eval p z).
+Proof.
+  simpl.
+  reflexivity.
+Qed.
+
+Lemma poly_eval_nil : forall (z : Z),
+  poly_eval nil z = 0.
+Proof.
+  intros.
+  simpl.
+  reflexivity.
+Qed.
+
+Lemma poly_eval_app : forall (p1 p2 : poly) (z : Z),
+  poly_eval (p1 ++ p2) z = poly_eval p1 z + (z^(Z.of_nat (length p1))) * (poly_eval p2 z).
 Proof.
   intros. induction p1.
-  - assert (Z.of_nat (Datatypes.length (nil:poly)) = 0).
-    { simpl. reflexivity. }
-    Search (nil ++ _). rewrite app_nil_l.
-    rewrite H. Search (_^0). rewrite Z.pow_0_r.
-    pose proof poly_eval'_nil z. rewrite H0.
+  - assert (Z.of_nat (Datatypes.length (nil:poly)) = 0). auto.
+    rewrite app_nil_l.
+    rewrite H. rewrite Z.pow_0_r.
+    pose proof poly_eval_nil z. rewrite H0.
     omega.
-  - Search (_ :: _ ++ _). rewrite <- app_comm_cons.
-    pose proof poly_eval'_cons (p1 ++ p2) a z.
+  - rewrite <- app_comm_cons.
+    pose proof poly_eval_cons (p1 ++ p2) a z.
     rewrite H. clear H. rewrite IHp1.
     rewrite Z.mul_add_distr_l.
     assert (z * (z ^ Z.of_nat (Datatypes.length p1)) = z ^ Z.of_nat (Datatypes.length (a :: p1))).
-    { Search (_ ^ 1). pose proof Z.pow_1_r z. rewrite <- H at 1.
-      Search (_ ^ _ * _ ^ _). pose proof Z.pow_add_r z 1 (Z.of_nat (Datatypes.length p1)).
-      assert (0 <= 1). { omega. }
+    {
+      pose proof Z.pow_1_r z. rewrite <- H at 1.
+      pose proof Z.pow_add_r z 1 (Z.of_nat (Datatypes.length p1)).
+      assert (0 <= 1). omega.
       assert (0 <= Z.of_nat (Datatypes.length p1)). 
-      { clear IHp1 H H0 H1.
+      {
+        clear IHp1 H H0 H1.
         induction p1.
         - simpl. omega.
-        - simpl. Search (0 <= Z.pos _).
-          apply Zle_0_pos.
-      } 
+        - simpl. apply Zle_0_pos.
+      }
       pose proof H0 H1 H2.
       rewrite <- H3.
       assert (1 + Z.of_nat (Datatypes.length p1) = Z.of_nat (Datatypes.length (a :: p1))).
-      { clear IHp1 H H0 H1 H2 H3.
-        Search (_ + Z.of_nat _). pose proof Nat2Z.inj_add 1 (length p1).
-        assert (Z.of_nat 1 = 1).
-        { simpl. omega. }
+      {
+        clear IHp1 H H0 H1 H2 H3.
+        pose proof Nat2Z.inj_add 1 (length p1).
+        assert (Z.of_nat 1 = 1). auto.
         rewrite <- H0.
         rewrite <- H.
-        Search (Z.of_nat _ = Z.of_nat _).
         pose proof inj_eq (1 + (length p1)) (length (a::p1)).
-        assert ((1 + Datatypes.length p1)%nat = Datatypes.length (a :: p1)).
-        { simpl. reflexivity. }
+        assert ((1 + Datatypes.length p1)%nat = Datatypes.length (a :: p1)). auto.
         omega.
       }
       rewrite H4.
       omega.
     }
     rewrite <- H.
-    pose proof poly_eval'_cons p1 a z.
+    pose proof poly_eval_cons p1 a z.
     rewrite H0.
-    Search (_ * (_ * _)).
     rewrite Z.mul_assoc.
     omega.
 Qed.
-    
-Theorem poly_eval_poly_eval' : forall (p : poly) (z : Z),
-  poly_eval p z = poly_eval' (rev p) z.
+
+Lemma poly_eval_add_zero_l: forall (p : poly) n z,
+  poly_eval (poly_add (repeat 0 n) p) z = poly_eval p z.
 Proof.
   intros.
-  induction p.
-  - simpl. reflexivity.
-  - simpl. pose proof poly_eval'_app (rev p) (a::nil) z.
-    rewrite H. simpl.
-    Search (_ * 0). rewrite Z.mul_0_r.
-    Search (_ + 0). rewrite Z.add_0_r.
-    Search (_ * _ = _ * _). rewrite Z.mul_comm.
-    Search (length (rev _) = length _). rewrite rev_length.
-    rewrite IHp. omega.
+  rewrite poly_add_spec.
+  rewrite poly_eval_zero.
+  omega.
 Qed.
 
-Theorem poly_eval_add_iso : forall p1 p2 z,
-  poly_eval (poly_add p1 p2) z = poly_eval p1 z + poly_eval p2 z.
+Lemma poly_eval_add_zero_r: forall (p : poly) n z,
+  poly_eval (poly_add p (repeat 0 n)) z = poly_eval p z.
 Proof.
   intros.
-  pose proof poly_eval_poly_eval' p1 z.
-  pose proof poly_eval_poly_eval' p2 z.
-  pose proof poly_eval_poly_eval' (poly_add p1 p2) z.
-  rewrite H. rewrite H0. rewrite H1.
-  unfold poly_add.
-  rewrite rev_involutive.
-  apply poly_eval'_add_body_iso.
+  rewrite poly_add_spec.
+  rewrite poly_eval_zero.
+  omega.
 Qed.
 
-Lemma poly_add_zero: forall (p : poly) times n,
-  poly_eval (poly_add (repeat 0 times) p) n = poly_eval p n.
-Proof.
-  intros.
-  induction p.
-  - simpl.
-    rewrite poly_add_empty_r.
-    rewrite poly_eval_0s.
-    reflexivity.
-  - simpl.
-    rewrite poly_eval_add_iso.
-    simpl.
-    rewrite poly_eval_0s.
-    omega.
-Qed.
-
-Lemma poly_add_body_comm: forall p1 p2,
-  poly_add_body p1 p2 = poly_add_body p2 p1.
+Lemma poly_add_comm: forall p1 p2,
+  poly_add p1 p2 = poly_add p2 p1.
 Proof.
   intro.
   induction p1; intros.
-  - rewrite poly_add_body_empty_l.
-    rewrite poly_add_body_empty_r.
-    reflexivity.
-  - induction p2.
-    + rewrite poly_add_body_empty_l.
-      rewrite poly_add_body_empty_r.
-      reflexivity.
+  - rewrite poly_add_nil_l, poly_add_nil_r. reflexivity.
+  - destruct p2.
+    + auto.
     + simpl.
       rewrite IHp1.
       rewrite Z.add_comm.
       reflexivity.
-Qed.
-
-Lemma poly_add_comm : forall p1 p2,
-  poly_add p1 p2 = poly_add p2 p1.
-Proof.
-  intros.
-  unfold poly_add.
-  rewrite poly_add_body_comm.
-  reflexivity.
-Qed.
-
-Lemma poly_add_body_cons_split : forall a p,
-  p ++ a :: nil = poly_add_body p ((repeat 0 (length p)) ++ a :: nil).
-Proof.
-  intros. revert a.
-  induction p; intros.
-  - simpl. reflexivity.
-  - simpl. rewrite <- IHp. rewrite Z.add_0_r. reflexivity.
-Qed.
-
-Lemma repeat_head_tail : forall (z : Z) n, z :: repeat z n = repeat z n ++ z :: nil.
-Proof.
-  intros.
-  induction n.
-  - auto.
-  - simpl. rewrite IHn. reflexivity.
-Qed.
-
-Lemma rev_repeat : forall (z : Z) n, rev (repeat z n) = repeat z n.
-Proof.
-  intros.
-  induction n.
-  - auto.
-  - simpl. rewrite IHn. rewrite repeat_head_tail. reflexivity.
-Qed.
-
-(* Lemma poly_add_body_same_level_tail : forall p1 p2 a1 a2,
-  length p1 = length p2 ->
-  poly_add_body (p1 ++ a1 :: nil) (p2 ++ a2 :: nil) = poly_add_body p1 p2 ++ (a1 + a2) :: nil.
-Proof.
-Admitted. *)
-
-Lemma poly_add_cons_split : forall a p,
-  a::p = poly_add (a :: (repeat 0 (length p))) p.
-Proof.
-  intros. revert a.
-  induction p; intros.
-  - simpl. rewrite poly_add_empty_r. reflexivity.
-  - unfold poly_add in *. simpl in *. rewrite rev_repeat in *.
-Admitted.
-
-Lemma poly_add_assoc : forall p1 p2 p3,
-  poly_add (poly_add p1 p2) p3 = poly_add p1 (poly_add p2 p3).
-Admitted.
-
-(* this is already proved in poly_eval_0s *)
-Lemma zero_poly : forall n z, poly_eval (repeat 0 n) z = 0.
-Proof.
-  apply poly_eval_0s.
-Qed.
-
-Lemma extract_single_term : forall a p z n, poly_eval (poly_add (a :: repeat 0 n) p) z = a * z ^ Z.of_nat n + poly_eval p z.
-Proof.
-  intros.
-  revert a. revert p.
-  induction n; intros.
-  - simpl. revert a.
-    induction p; intros.
-    + simpl. reflexivity.
-    + simpl.
-  (*
-  revert a. revert n.
-  induction p; intros.
-  - rewrite poly_add_empty_r. simpl. rewrite zero_poly, repeat_length. reflexivity.
-  - Admitted.*) Admitted.
-
-Lemma poly_add_eval_comm : forall p1 p2 z,
-  poly_eval (poly_add p1 p2) z = poly_eval p1 z + poly_eval p2 z.
-(* rename it for code consistency
-**)
-Proof.
-  apply poly_eval_add_iso.
 Qed.
 (** [] *)
 
@@ -456,33 +339,11 @@ Inductive loosen : AsymptoticBound -> AsymptoticBound -> Prop :=
   | Theta2Omega : forall p n, BigTheta p n =< BigOmega p n
   | Theta2O : forall p n, BigTheta p n =< BigO p n
   | HighestEquivO : forall p1 p2 n,
-                      length (trim_0_l p1) = length (trim_0_l p2) ->
+                      length (trim_0 p1) = length (trim_0 p2) ->
                       BigO p1 n =< BigO p2 n
   (* TODO: more highest equiv loosenings *)
   (* TODO: other loosenings *)
   
   where "T1 '=<' T2" := (loosen T1 T2).
-
-
-(** This rule is invalid *)
-(*
-Theorem loosen_valid :
-  forall T1 T2, T1 =< T2 ->
-  forall t, (exists (a1 a2 N : Z), 0 < a1 -> 0 < a2 -> 0 < N ->
-    forall La, ab_eval La T1 a1 a2 N t) ->
-  exists (a1' a2' N' : Z), 0 < a1' -> 0 < a2' -> 0 < N' ->
-    forall La, ab_eval La T2 a1' a2' N' t.
-Proof.
-  intros. revert H0.
-  induction H; intros [a1 [a2 [N ?]]]; simpl in *;
-  try (exists a1, a2, N;
-      intros;
-      pose proof H H0 H1 H2 La H3; omega).
-  (* Prove the polynomial asymptotic bounds are equivalent when the highest orders are the same *)
-  - (* HighestEquivTheta *)
-    simpl in *.
-    
-  Admitted.
-*)
 
 End Polynomial_Asympotitic_Bound.
