code/Denotation.v
@@ -1,79 +1,21 @@
 Require Import Coq.Lists.List.
 Require Import AB.Imp8.
 
-(* ################################################################# *)
-(** * Review: Denotations *)
-(*
-Module Expression_Denotation.
-
-Fixpoint aeval (a : aexp) (st : state) : Z :=
-  match a with
-  | ANum n => n
-  | AId X => st X
-  | APlus a1 a2 => (aeval a1 st) + (aeval a2 st)
-  | AMinus a1 a2  => (aeval a1 st) - (aeval a2 st)
-  | AMult a1 a2 => (aeval a1 st) * (aeval a2 st)
-  end.
-
-Fixpoint beval (b : bexp) (st : state) : Prop :=
-  match b with
-  | BTrue       => True
-  | BFalse      => False
-  | BEq a1 a2   => (aeval a1 st) = (aeval a2 st)
-  | BLe a1 a2   => (aeval a1 st) <= (aeval a2 st)
-  | BNot b1     => ~ (beval b1 st)
-  | BAnd b1 b2  => (beval b1 st) /\ (beval b2 st)
-  end.
-
-End Expression_Denotation.
-
-Module Relation_Operators.
-
-Definition id {A: Type}: A -> A -> Prop := fun a b => a = b.
-
-Definition empty {A B: Type}: A -> B -> Prop := fun a b => False.
-
-Definition concat {A B C: Type} (r1: A -> B -> Prop) (r2: B -> C -> Prop): A -> C -> Prop :=
-  fun a c => exists b, r1 a b /\ r2 b c.
-
-Definition filter1 {A B: Type} (f: A -> Prop): A -> B -> Prop :=
-  fun a b => f a.
-
-Definition filter2 {A B: Type} (f: B -> Prop): A -> B -> Prop :=
-  fun a b => f b.
-
-Definition union {A B: Type} (r1 r2: A -> B -> Prop): A -> B -> Prop :=
-  fun a b => r1 a b \/ r2 a b.
-
-Definition intersection {A B: Type} (r1 r2: A -> B -> Prop): A -> B -> Prop :=
-  fun a b => r1 a b /\ r2 a b.
-
-Definition omega_union {A B: Type} (rs: nat -> A -> B -> Prop): A -> B -> Prop :=
-  fun st1 st2 => exists n, rs n st1 st2.
-
-End Relation_Operators.
-*)
 Module Command_Denotation_With_Steps.
 
-(*Import Expression_Denotation.*)
-
-(** This time, a program's denotation is defined as a trinary relation.
-Specifically, [st1, t, st2] belongs to the denotation of program [c] if and
-only if executing [c] from [st1] may take time [t] and stop at state [st2]. *)
+(* Here we assume that every command will cost time, more specifically, SKIP command should take 1 time steps instead of 0. *)
 
 Definition skip_sem: state -> Z -> state -> Prop :=
   fun st1 t st2 =>
-    st1 = st2 /\ t = 1. (* <-- modified *)
+    st1 = st2 /\ t = 1.                             (* <-- modified *)
+
+(* Originally the t is dependent with Y, here we move t out and is an independent conjunction branch. *)
 
 Definition asgn_sem (X: var) (E: aexp): state -> Z -> state -> Prop :=
   fun st1 t st2 =>
     st2 X = aeval E st1 /\
-    (forall Y, X <> Y -> st1 Y = st2 Y) /\ (* <-- modified *)
+    (forall Y, X <> Y -> st1 Y = st2 Y) /\          (* <-- modified *)
     t = 1.
-
-(** Here we assume every assignment command takes one unit of time. We can
-write a more realistic definition here so that different assignment commands
-may take different amount of time. *)
 
 Definition seq_sem (d1 d2: state -> Z -> state -> Prop)
   : state -> Z -> state -> Prop
@@ -88,8 +30,6 @@ Definition if_sem (b: bexp) (d1 d2: state -> Z -> state -> Prop)
   fun st1 t st2 =>
     (d1 st1 (t - 1) st2 /\ beval b st1) \/
     (d2 st1 (t - 1) st2 /\ ~beval b st1).
-
-(** Here we assume that testing an if-condition will take one unit of time. *)
 
 Fixpoint iter_loop_body
   (b: bexp)
@@ -109,8 +49,6 @@ Fixpoint iter_loop_body
          t = t1 + t2) /\
        beval b st1
   end.
-
-(** Here we assume that testing a loop condition will take one unit of time. *)
 
 Definition loop_sem (b: bexp) (loop_body: state -> Z -> state -> Prop)
   : state -> Z -> state -> Prop
